improved error messages and fixed proof

src/arch/x64/X64.Vale.StrongPost_i.fsti
@@ -32,16 +32,29 @@ unfold let va_fast_ins_Sub64 = Sub64
 
 unfold let va_inss = list ins
 
-let valid_maddr_norm (r:range) (addr:maddr) (s:state) : Type0 =
-  labeled r (string_of_maddr addr)
-	    (Map.contains s.mem (eval_maddr addr s))
+let valid_maddr_norm (addr:maddr) (s:state) : bool =
+  Map.contains s.mem (eval_maddr addr s)
+ 
+let valid_maddr (r:range) (addr:maddr) (s:state) : Type0 =
+  let msg = normalize_term (
+      strcat (strcat ("Memory address ") (string_of_maddr addr))
+	     (" is invalid")) in
+  labeled r msg
+	  (valid_maddr_norm addr s)
 
-let valid_operand_norm (r:range) (o:operand) (s:state) : Type0 =
+let valid_operand_norm (o:operand) (s:state) : bool =
+  match o with
+  | OConst n -> 0 <= n && n < nat64_max
+  | OReg r -> true
+  | OMem m -> valid_maddr_norm m s
+
+let valid_operand (r:range) (o:operand) (s:state)  =
   labeled r "Failed to prove that the operand is valid"
     (match o with
     | OConst n -> b2t (0 <= n && n < nat64_max)
     | OReg r -> True
-    | OMem m -> valid_maddr_norm r m s)
+    | OMem m -> valid_maddr r m s)
+
 
 let eval_operand_norm (o:operand) (s:state) : nat64 =
   match o with
@@ -105,71 +118,71 @@ let rec wp_code (inss : list ins) (post: state -> Type0) (s0:state) : Type0 =
       match hd with
       | (Mov64 (OReg Rsp) _) -> False
       | (Mov64 (OReg dst) src) ->
-	valid_operand_norm r_info src s0 /\
+	valid_operand r_info src s0 /\
 	(forall x. x == eval_operand_norm src s0 ==>
               wp_code inss post (update_reg dst x s0))
       | (Load64 (OReg Rsp) _ _) -> False
       | (Load64 (OReg dst) (OReg src) offset) ->
-	  valid_maddr_norm r_info (MReg src offset) s0 /\
-	(forall x. x == Map.sel s0.mem (s0.regs src + offset) ==>
+      	  valid_maddr r_info (MReg src offset) s0 /\
+      	(forall x. x == Map.sel s0.mem (s0.regs src + offset) ==>
               wp_code inss post (update_reg dst x s0))
       | (Store64 (OReg dst) src offset) ->
-	(valid_operand_norm r_info src s0) /\
-	(Map.contains s0.mem (s0.regs dst + offset)) /\
-	(forall x.
-	  x == Map.upd s0.mem (s0.regs dst + offset) (eval_operand_norm src s0) ==>
-	  wp_code inss post ({s0 with mem = x}))
+      	(valid_operand r_info src s0) /\
+      	(Map.contains s0.mem (s0.regs dst + offset)) /\
+      	(forall x.
+      	  x == Map.upd s0.mem (s0.regs dst + offset) (eval_operand_norm src s0) ==>
+      	  wp_code inss post ({s0 with mem = x}))
       | (Add64Wrap (OReg Rsp) _) -> False
       | (Add64Wrap (OReg dst) src) ->
-	(valid_operand_norm r_info src s0) /\
-	(forall a x (f:nat64).
-	     a == s0.regs dst + eval_operand_norm src s0 /\
-	     x == (if a < nat64_max then a else a - nat64_max) /\
-		  cf f == (a >= nat64_max) ==>
-	       wp_code inss post ({update_reg dst x s0 with flags = f}))
+      	(valid_operand r_info src s0) /\
+      	(forall a x (f:nat64).
+      	     a == s0.regs dst + eval_operand_norm src s0 /\
+      	     x == (if a < nat64_max then a else a - nat64_max) /\
+      		  cf f == (a >= nat64_max) ==>
+      	       wp_code inss post ({update_reg dst x s0 with flags = f}))
       | (Adc64Wrap (OReg Rsp) _) -> False
       | (Adc64Wrap (OReg dst) src) ->
-	(valid_operand_norm r_info src s0) /\
-	(forall a x (f:nat64).
-	     a == s0.regs dst + eval_operand_norm src s0 + 
-		  (if cf s0.flags then 1 else 0) /\
-	     x == (if a < nat64_max then a else a - nat64_max) /\
-		   cf f == (a >= nat64_max) ==>
-	       wp_code inss post ({update_reg dst x s0 with flags = f}))
+      	(valid_operand r_info src s0) /\
+      	(forall a x (f:nat64).
+      	     a == s0.regs dst + eval_operand_norm src s0 + 
+      		  (if cf s0.flags then 1 else 0) /\
+      	     x == (if a < nat64_max then a else a - nat64_max) /\
+      		   cf f == (a >= nat64_max) ==>
+      	       wp_code inss post ({update_reg dst x s0 with flags = f}))
       | (Mul64Wrap src) ->
-	(valid_operand_norm r_info src s0) /\
-	(forall (rax:nat64) (rdx:nat64) (f:nat64).
-	  nat64_max `op_Multiply` rdx + rax == 
-		    s0.regs Rax `op_Multiply` eval_operand_norm src s0 ==>
-	    wp_code inss post (update_reg Rdx rdx (update_reg Rax rax 
-							      ({s0 with flags = f}))))
+      	(valid_operand r_info src s0) /\
+      	(forall (rax:nat64) (rdx:nat64) (f:nat64).
+      	  nat64_max `op_Multiply` rdx + rax == 
+      		    s0.regs Rax `op_Multiply` eval_operand_norm src s0 ==>
+      	    wp_code inss post (update_reg Rdx rdx (update_reg Rax rax 
+      							      ({s0 with flags = f}))))
       | (IMul64 (OReg Rsp) _) -> False
       | (IMul64 (OReg dst) src) ->
-	let a = s0.regs dst `op_Multiply` eval_operand_norm src s0 in
-	  (valid_operand_norm r_info src s0) /\
-	  (a < nat64_max) /\ //TODO:label this
-	  (forall (x:nat64) (f:nat64).
-	     x == a ==>
-	       wp_code inss post ({update_reg dst x s0 with flags = f}))
+      	let a = s0.regs dst `op_Multiply` eval_operand_norm src s0 in
+      	  (valid_operand r_info src s0) /\
+      	  (a < nat64_max) /\ //TODO:label this
+      	  (forall (x:nat64) (f:nat64).
+      	     x == a ==>
+      	       wp_code inss post ({update_reg dst x s0 with flags = f}))
       | (And64 (OReg Rsp) _) -> False
       | (And64 (OReg dst) src) ->
-	let a = logand64 (s0.regs dst) (eval_operand_norm src s0) in
-	(valid_operand_norm r_info src s0) /\
-	(forall (x:nat64) (f:nat64).
-	  x == a ==>
-	  wp_code inss post ({update_reg dst x s0 with flags = f}))
+      	let a = logand64 (s0.regs dst) (eval_operand_norm src s0) in
+      	(valid_operand r_info src s0) /\
+      	(forall (x:nat64) (f:nat64).
+      	  x == a ==>
+      	  wp_code inss post ({update_reg dst x s0 with flags = f}))
       | (Shr64 (OReg Rsp) _) -> False
       | (Shr64 (OReg dst) src) ->
-	let a = shift_right64 (s0.regs dst) (eval_operand_norm src s0) in
-	(valid_operand_norm r_info src s0) /\
-	(forall (x:nat64) (f:nat64).
-	  x == a ==>
-	  wp_code inss post ({update_reg dst x s0 with flags = f}))
+      	let a = shift_right64 (s0.regs dst) (eval_operand_norm src s0) in
+      	(valid_operand r_info src s0) /\
+      	(forall (x:nat64) (f:nat64).
+      	  x == a ==>
+      	  wp_code inss post ({update_reg dst x s0 with flags = f}))
       | (Sub64 (OReg Rsp) _) -> False
       | (Sub64 (OReg dst) src) ->
-	       (valid_operand_norm r_info src s0) /\
-	       (0 <= s0.regs dst - eval_operand_norm src s0) /\
-	       (forall a x (f:nat64).
+      	       (valid_operand r_info src s0) /\
+      	       (0 <= s0.regs dst - eval_operand_norm src s0) /\
+      	       (forall a x (f:nat64).
                a == s0.regs dst - eval_operand_norm src s0 /\
                x == a ==>
                wp_code inss post ({update_reg dst x s0 with flags = f}))
@@ -190,6 +203,8 @@ let wp_code_delta = [
   "X64.Vale.State_i.__proj__Mkstate__item__mem";
   "X64.Vale.StrongPost_i.valid_operand_norm";
   "X64.Vale.StrongPost_i.valid_maddr_norm";
+  "X64.Vale.StrongPost_i.valid_operand";
+  "X64.Vale.StrongPost_i.valid_maddr";
   "X64.Machine_s.string_of_maddr";
   "X64.Machine_s.string_of_reg";
   "X64.Vale.StrongPost_i.augment"
@@ -214,7 +229,7 @@ val va_lemma_weakest_pre_norm (inss:list ins) (s0:state) (sN:state) : PURE unit
 (* #reset-options "--log_queries --debug X64.Vale.StrongPost_i --debug_level print_normalized_terms" *)
 let test_lemma (s0:state) (sN:state) =
     assume (s0.ok);
-    // assume (Map.contains s0.mem (s0.regs Rsi));
+    //assume (Map.contains s0.mem (s0.regs Rsi));
     assume (Map.contains s0.mem (s0.regs Rcx));
     let i1 = Prims.set_range_of (Load64 (OReg Rax) (OReg Rsi) 0)
                                 (mk_range "load-instruction-1" 1 1 2 0) in
