src/arch/x64/X64.Vale.StrongPost_i.fst
@@ -29,6 +29,20 @@ let assert_to_norm' (p:Type0): Lemma
   (ensures (Prims.norm [delta_only wp_code_delta; zeta; iota; primops] p))
   = ()
 
+let lemma_valid_maddr_eq (r:range) (addr:maddr) (s:state) :
+  Lemma (valid_maddr_norm addr s <==> valid_maddr r addr s) =
+    assert_from_norm' (valid_maddr_norm addr s <==> valid_maddr r addr s)
+
+let lemma_valid_op_eq (r:range) (op:operand) (s:state) :
+  Lemma (valid_operand_norm op s <==> valid_operand r op s) =
+   let _ =  match op with
+	    | OConst n -> ()
+	    | OReg r -> ()
+	    | OMem m -> lemma_valid_maddr_eq r m s
+   in
+     assert_from_norm' (valid_operand_norm op s <==> valid_operand r op s)
+
+
 let lemma_weak_pre_ins (i:ins) (inss:list ins) 
 			       (s0:state) (sN:state) (post: unit -> Type) :
   Ghost (option state)
@@ -52,44 +66,52 @@ let lemma_weak_pre_ins (i:ins) (inss:list ins)
     Some sM
   in*)
   let _ = assert_to_norm'(wp_code (i::inss) (augment sN post) s0) in
+  let r_info = range_of i in
   match i with
   | Mov64 (OReg dst) src ->
+    let _ = lemma_valid_op_eq r_info src s0 in
       if dst <> Rsp && valid_operand_norm src s0 then
         let (bM, sM) = va_lemma_Mov64 b0 s0 sN (OReg dst) src in
 	  Some sM
       else 
 	  None
   | Load64 (OReg dst) (OReg src) offset ->
-      if dst <> Rsp && valid_src_addr s0.mem (s0.regs src + offset) then
+    let _ = lemma_valid_maddr_eq r_info (MReg src offset) s0 in
+      if dst <> Rsp && valid_maddr_norm (MReg src offset) s0 then
         let (bM, sM) = va_lemma_Load64 b0 s0 sN (OReg dst) (OReg src) offset in
   	  Some sM
       else
   	  None
   | Store64 (OReg dst) src offset ->
+    let _ = lemma_valid_op_eq r_info src s0 in
       if valid_dst_addr s0.mem (s0.regs dst + offset) && valid_operand_norm src s0 then
         let (bM, sM) = va_lemma_Store64 b0 s0 sN (OReg dst) src offset in
   	  Some sM
       else
   	  None
   | Add64Wrap (OReg dst) src ->
+    let _ = lemma_valid_op_eq r_info src s0 in
       if dst <> Rsp && valid_operand_norm src s0 then
         let (bM, sM) = va_lemma_Add64Wrap b0 s0 sN (OReg dst) src in
   	  Some sM
       else
   	  None
   | Adc64Wrap (OReg dst) src ->
+    let _ = lemma_valid_op_eq r_info src s0 in
       if dst <> Rsp && valid_operand_norm src s0 then
         let (bM, sM) = va_lemma_Adc64Wrap b0 s0 sN (OReg dst) src in
   	  Some sM
       else
   	  None
   | Mul64Wrap src ->
+    let _ = lemma_valid_op_eq r_info src s0 in
       if valid_operand_norm src s0 then
         let (bM, sM) = va_lemma_Mul64Wrap b0 s0 sN src in
   	  Some sM
       else
   	  None
   | IMul64 (OReg dst) src ->
+      lemma_valid_op_eq r_info src s0;
       let a = s0.regs dst `op_Multiply` eval_operand_norm src s0 in
       if dst <> Rsp && valid_operand_norm src s0 && a < nat64_max then
         let (bM, sM) = va_lemma_IMul64 b0 s0 sN (OReg dst) src in
@@ -97,6 +119,7 @@ let lemma_weak_pre_ins (i:ins) (inss:list ins)
       else
   	  None
   | And64 (OReg dst) src ->
+    lemma_valid_op_eq r_info src s0;
     let a = logand64 (s0.regs dst) (eval_operand_norm src s0) in
     if dst <> Rsp && valid_operand_norm src s0 then
       let (bM, sM) = va_lemma_And64 b0 s0 sN (OReg dst) src in
@@ -104,6 +127,7 @@ let lemma_weak_pre_ins (i:ins) (inss:list ins)
       else
   	  None
   | Shr64 (OReg dst) src ->
+    lemma_valid_op_eq r_info src s0;
     let a = shift_right64 (s0.regs dst) (eval_operand_norm src s0) in
     if dst <> Rsp && valid_operand_norm src s0 then
       let (bM, sM) = va_lemma_Shr64 b0 s0 sN (OReg dst) src in
@@ -111,8 +135,9 @@ let lemma_weak_pre_ins (i:ins) (inss:list ins)
       else
   	  None
   | Sub64 (OReg dst) src ->
+    lemma_valid_op_eq r_info src s0;
     if dst <> Rsp && valid_operand_norm src s0 && 0 <= 
-		    (s0.regs dst) - (eval_operand_norm src s0) then
+  		    (s0.regs dst) - (eval_operand_norm src s0) then
       let (bM, sM) = va_lemma_Sub64 b0 s0 sN (OReg dst) src in
   	  Some sM
       else
